examples/map/MapIAproof.v
@@ -5,7 +5,7 @@ Require Import MapHeader MapA MapM MapI ModSim MapIMproof MapMAproof MemA wsim.
 Module MapIA. Section MapIA.
   Context `{!invG α Σ Γ, !subG Γ Σ, !sinvG Σ Γ α β τ, !MapAGΓ Γ, !MapMGΓ Γ, !memGΓ Γ}.
 
-  Lemma wctxr (u_s u_mem : univ_id) (spc_s spc_mem : string → option fspec)
+  Lemma ctxr (u_s u_mem : univ_id) (spc_s spc_mem : string → option fspec)
       (LE : u_s >= 2)
       (MapInSpcMap : spc_incl (MapAS.spc u_s) spc_s) :
     ctx_refines
@@ -13,11 +13,11 @@ Module MapIA. Section MapIA.
       ((MapI.t)           ★ (MemA.t u_mem spc_mem), emp%I).
   Proof.
     etrans; cycle 1.
-    { eapply MapIM.wctxr.
+    { eapply MapIM.ctxr.
       instantiate (1:= to_spc (MapMS.spc 1)).
       i. split; try refl. unfold MapMS.spc. unseal CRIS. prove_nodup.
     }
     eapply ctxr_frameR. rewrite -(hmod_addc_empty_l (MapM.t _ _)). eapply ctxr_cond_frameR.
-    eapply MapMA.wctxr; eauto. rewrite /MapMS.spc; unseal CRIS; prove_nodup. ss.
+    eapply MapMA.ctxr; eauto. rewrite /MapMS.spc; unseal CRIS; prove_nodup. ss.
   Qed.
 End MapIA. End MapIA.
