examples/mutsum/MutGIAproof.v
@@ -88,10 +88,10 @@ Module MutGIA. Section MutGIA.
   Qed.
 End MutGIA.
 
-Section wctxr.
+Section ctxr.
   Context `{!invG α Σ Γ, !subG Γ Σ, !sinvG Σ Γ α β τ}.
 
-  Theorem wctxr (u_s u_apc: univ_id) (Spc SpcPure: string → option fspec) 
+  Theorem ctxr (u_s u_apc: univ_id) (Spc SpcPure: string → option fspec) 
     (APCInSpc : spc_incl (APCA.Spc) Spc)
     (FInPure : spc_incl (MutFA.SpcF) SpcPure)
     (PureInSpc : spc_sub SpcPure Spc)
@@ -100,4 +100,4 @@ Section wctxr.
       (MutGA.t u_s Spc ★ APCA.t u_apc SpcPure Spc, MutGA.InitCond)
       (MutGI.t ★ APCA.t u_apc SpcPure Spc, emp%I).
   Proof. eapply main_adequacy, sim; eauto. Qed.
-End wctxr. End MutGIA.
+End ctxr. End MutGIA.
